SStructTT.lean
@@ -54,6 +54,6 @@ import SStructTT.SStruct.Erasure.Preservation
 import SStructTT.SStruct.Erasure.Progress
 import SStructTT.SStruct.Erasure.Normalize
 
--- import SStructTT.SStruct.Runtime.Heap
--- import SStructTT.SStruct.Runtime.Resolution
+import SStructTT.SStruct.Runtime.Heap
+import SStructTT.SStruct.Runtime.Resolution
 -- import SStructTT.SStruct.Runtime.Step
